add blood list class and add remove method

verification/BloodList.dfy
@@ -1,14 +1,97 @@
+class {:autocontracts} BloodList
+{
+  var list: array<int>;
+  var upto: int;
+
+  ghost var bloodSet: set<int>;
+
+  predicate Valid()
+  reads this;
+  {
+    list != null && 0 <= upto < list.Length
+    //&& forall x :: x in bloodSet ==> exists t :: 0 <= t <= upto && list[t] == x
+  }
+
+  constructor(size: int)
+  // modifies this;
+  requires size > 0;
+  // ensures Valid();
+  ensures fresh(list);
+  {
+    list := new int[size];
+    upto := 0;
+    bloodSet := {};
+  }
+
+  method addBlood(blood: int)
+  // requires Valid(); ensures Valid();
+  ensures list[upto] == blood;
+  ensures upto == old(upto) + 1;
+  ensures old(list[0..old(upto)]) == list[0..old(upto)];
+  ensures bloodSet == old(bloodSet) + {blood};
+  {
+    // assert forall x :: x in bloodSet ==> exists t :: 0 <= t <= upto && list[t] == x;
+   
+    bloodSet := bloodSet + {blood};
+    if upto == list.Length - 1
+    {
+      var newlist := new int[2*list.Length];
+      forall(i | 0 <= i < list.Length)
+      { 
+        newlist[i] := list[i];
+      }
+      list := newlist;
+    }
+    list[upto+1], upto := blood, upto + 1;
+
+    // assert blood in bloodSet && list[upto] == blood;
+    // assert forall x :: x in bloodSet ==> exists t :: 0 <= t <= upto && list[t] == x;
+
+  }
+
+  method removeBlood(blood: int)
+  // requires Valid(); ensures Valid();
+  requires upto > 0;
+  requires blood in bloodSet;
+  requires exists t :: 0 <= t <= upto && list[t] == blood;
+  ensures upto == old(upto) - 1;
+  ensures bloodSet == old(bloodSet) - {blood};
+  {
+    var i:=0;
+
+    while i <= upto
+    invariant 0 <= i <= upto;
+    invariant forall k :: 0 <= k < i ==> list[k] != blood;
+    decreases upto - i;
+    {
+      if list[i]==blood
+      {
+          forall(j | i < j <= upto) 
+          {
+            list[j - 1] := list[j];
+          }
+          bloodSet := bloodSet - {blood};
+          break;
+      }
+      i := i + 1;
+    }
+    upto := upto - 1;
+  }
+}
+
 
 // haven't complete verifying this part
-method addBlood(a:seq<int>,id:int) returns (b:seq<int>)
+/*method addBlood(a:seq<int>,id:int) returns (a:seq<int>)
+  requires |a| > 0
+  ensures id in a
 { 
-  b := a + [id];
+  a := a + [id];
 }
 
 
 method RemoveBlood(a:seq<int>, id:int)returns (b:seq<int>)
   requires |a|>0
-  ensures id !in a ==> a ==b;
+  ensures id !in a ==> a == b;
  // ensures forall k :: 0<=k<|b| ==> (b[k]!=id);
 {
  var i:=0;
@@ -54,4 +137,4 @@ method Main() {
   print n;
   print "\n";
   assert n==s;
-}
+}*/
